Proofs/TypeSystem.v
@@ -9,7 +9,6 @@ Require Import Definitions.Tactics.
 Require Import Proofs.LocallyNameless.
 Require Import Definitions.GHeap. 
 Require Import Proofs.Determinism.
-Require Import Definitions.Axioms.
 Require Import Definitions.GTypes.
 Require Import Definitions.DynamicActions.
 Require Import Proofs.EffectFacts.
@@ -162,28 +161,536 @@ Lemma TcValExtended_2:
     TcVal (stty ∪ (stty1 ∖ stty ∪ stty2 ∖ stty), Pair (v1, v2),
         subst_rho rho (Ty_Pair ty1 ty2)).
 Proof.
-  intros.
+  intros stty stty1 stty2 v1 v2 rho ty1 ty2
+    Hdisj Hext1 Hext2 HTcVal1 HTcVal2.
   replace (subst_rho rho (Ty_Pair ty1 ty2))
     with (Ty_Pair (subst_rho rho ty1) (subst_rho rho ty2))
     by (now rewrite subst_rho_pair).
   econstructor; eauto.
-  - apply ext_stores__val with (stty:=stty1). intros.
-     + apply StoreTyping_Union; auto.
-       * apply map_disjoint_union_r.
-         { split.
-           - apply map_disjoint_difference_r.
-             now apply WeakenigImpliesSubsetEq.
-           - apply map_disjoint_difference_r.
-             now apply WeakenigImpliesSubsetEq.}
-       * right.
-         apply StoreTyping_Union; auto.
-         left.
-         { apply lookup_difference_Some. split.
-           - assumption.
-           - admit.               
-         }
-     + assumption.
-Admitted.
+  - apply ext_stores__val with (stty:=stty1).
+    + intros l t' Hfind.
+      unfold find_ST in *.
+      apply lookup_union_Some_raw.
+      destruct (stty !! l) eqn:Hbase.
+      * left.
+        apply Hext1 in Hbase.
+        unfold find_ST in Hbase.
+        rewrite Hfind in Hbase.
+        inversion Hbase; subst.
+        assumption.
+      * right. split; [reflexivity |].
+        apply lookup_union_Some_raw.
+        left.
+        apply lookup_difference_Some.
+        split.
+        -- assumption.
+        -- rewrite Hbase. reflexivity.
+    + assumption.
+  - apply ext_stores__val with (stty:=stty2).
+    + intros l t' Hfind.
+      unfold find_ST in *.
+      apply lookup_union_Some_raw.
+      destruct (stty !! l) eqn:Hbase.
+      * left.
+        apply Hext2 in Hbase.
+        unfold find_ST in Hbase.
+        rewrite Hfind in Hbase.
+        inversion Hbase; subst.
+        assumption.
+      * right. split; [reflexivity |].
+        assert (Hdiff2 : (stty2 ∖ stty) !! l = Some t').
+        { apply lookup_difference_Some. split.
+          - assumption.
+          - rewrite Hbase. reflexivity. }
+        apply lookup_union_Some_raw.
+        right. split; [| assumption].
+        assert (Hdisj_spec : forall i x y,
+                   (stty1 ∖ stty) !! i = Some x ->
+                   (stty2 ∖ stty) !! i = Some y -> False)
+          by (apply map_disjoint_spec; assumption).
+        destruct ((stty1 ∖ stty) !! l) eqn:Hdiff1; auto.
+        exfalso. eapply Hdisj_spec; eauto.
+    + assumption.
+Qed.
+
+Inductive Phi_Updates : SigmaKey -> Val -> Phi -> Prop :=
+| PU_Alloc : forall r l v,
+    Phi_Updates (r, l) v (Phi_Elem (DA_Alloc r l v))
+| PU_Write : forall r l v,
+    Phi_Updates (r, l) v (Phi_Elem (DA_Write r l v))
+| PU_Seq_L : forall k v phi1 phi2,
+    Phi_Updates k v phi1 ->
+    Phi_Updates k v (Phi_Seq phi1 phi2)
+| PU_Seq_R : forall k v phi1 phi2,
+    Phi_Updates k v phi2 ->
+    Phi_Updates k v (Phi_Seq phi1 phi2)
+| PU_Par_L : forall k v phi1 phi2,
+    Phi_Updates k v phi1 ->
+    Phi_Updates k v (Phi_Par phi1 phi2)
+| PU_Par_R : forall k v phi1 phi2,
+    Phi_Updates k v phi2 ->
+    Phi_Updates k v (Phi_Par phi1 phi2).
+
+Inductive Phi_Allocates : SigmaKey -> Phi -> Prop :=
+| PA_Alloc : forall r l v,
+    Phi_Allocates (r, l) (Phi_Elem (DA_Alloc r l v))
+| PA_Seq_L : forall k phi1 phi2,
+    Phi_Allocates k phi1 ->
+    Phi_Allocates k (Phi_Seq phi1 phi2)
+| PA_Seq_R : forall k phi1 phi2,
+    Phi_Allocates k phi2 ->
+    Phi_Allocates k (Phi_Seq phi1 phi2)
+| PA_Par_L : forall k phi1 phi2,
+    Phi_Allocates k phi1 ->
+    Phi_Allocates k (Phi_Par phi1 phi2)
+| PA_Par_R : forall k phi1 phi2,
+    Phi_Allocates k phi2 ->
+    Phi_Allocates k (Phi_Par phi1 phi2).
+
+Definition TcPhi (stty : Sigma) (phi : Phi) : Prop :=
+  forall k v,
+    Phi_Updates k v phi ->
+    exists t, find_ST k stty = Some t /\ TcVal (stty, v, t).
+
+Lemma Phi_Updates_nil_false :
+  forall k v, ~ Phi_Updates k v Phi_Nil.
+Proof.
+  intros k v H. inversion H.
+Qed.
+
+Lemma Phi_Allocates_nil_false :
+  forall k, ~ Phi_Allocates k Phi_Nil.
+Proof.
+  intros k H. inversion H.
+Qed.
+
+Lemma TcPhi_nil :
+  forall stty, TcPhi stty Phi_Nil.
+Proof.
+  unfold TcPhi. intros stty k v H. inversion H.
+Qed.
+
+Lemma TcPhi_weaken :
+  forall stty stty' phi,
+    (forall k t, find_ST k stty = Some t -> find_ST k stty' = Some t) ->
+    TcPhi stty phi ->
+    TcPhi stty' phi.
+Proof.
+  unfold TcPhi.
+  intros stty stty' phi Hweak HTcPhi k v HUpdate.
+  destruct (HTcPhi k v HUpdate) as [t [Hfind HTcVal]].
+  exists t. split; [now apply Hweak |].
+  eapply ext_stores__val; eauto.
+Qed.
+
+Lemma TcPhi_seq :
+  forall stty phi1 phi2,
+    TcPhi stty phi1 ->
+    TcPhi stty phi2 ->
+    TcPhi stty (Phi_Seq phi1 phi2).
+Proof.
+  unfold TcPhi.
+  intros stty phi1 phi2 H1 H2 k v HUpdate.
+  inversion HUpdate; subst; eauto.
+Qed.
+
+Lemma TcPhi_par :
+  forall stty phi1 phi2,
+    TcPhi stty phi1 ->
+    TcPhi stty phi2 ->
+    TcPhi stty (Phi_Par phi1 phi2).
+Proof.
+  unfold TcPhi.
+  intros stty phi1 phi2 H1 H2 k v HUpdate.
+  inversion HUpdate; subst; eauto.
+Qed.
+
+Lemma StoreTyping_Extended_Base :
+  forall l t (stty stty1 stty2 : Sigma),
+    stty1 ∖ stty ##ₘ stty2 ∖ stty ->
+    (forall k t', find_ST k stty = Some t' -> find_ST k stty1 = Some t') ->
+    (forall k t', find_ST k stty = Some t' -> find_ST k stty2 = Some t') ->
+    find_ST l stty = Some t ->
+    find_ST l (stty ∪ (stty1 ∖ stty ∪ stty2 ∖ stty)) = Some t.
+Proof.
+  intros.
+  eapply StoreTyping_Union_2; eauto.
+Qed.
+
+Lemma StoreTyping_Extended_Left :
+  forall l t (stty stty1 stty2 : Sigma),
+    stty1 ∖ stty ##ₘ stty2 ∖ stty ->
+    (forall k t', find_ST k stty = Some t' -> find_ST k stty1 = Some t') ->
+    find_ST l stty1 = Some t ->
+    find_ST l (stty ∪ (stty1 ∖ stty ∪ stty2 ∖ stty)) = Some t.
+Proof.
+  intros l t stty stty1 stty2 Hdisj Hext Hfind.
+  unfold find_ST in *.
+  apply lookup_union_Some_raw.
+  destruct (stty !! l) eqn:Hbase.
+  - left.
+    assert (Hbase_ext := Hbase).
+    apply Hext in Hbase_ext.
+    unfold find_ST in Hbase_ext.
+    rewrite Hfind in Hbase_ext.
+    inversion Hbase_ext; subst.
+    assumption.
+  - right. split; [exact Hbase |].
+    apply lookup_union_Some_raw.
+    left.
+    apply lookup_difference_Some. split; auto.
+Qed.
+
+Lemma StoreTyping_Extended_Right :
+  forall l t (stty stty1 stty2 : Sigma),
+    stty1 ∖ stty ##ₘ stty2 ∖ stty ->
+    (forall k t', find_ST k stty = Some t' -> find_ST k stty2 = Some t') ->
+    find_ST l stty2 = Some t ->
+    find_ST l (stty ∪ (stty1 ∖ stty ∪ stty2 ∖ stty)) = Some t.
+Proof.
+  intros l t stty stty1 stty2 Hdisj Hext Hfind.
+  unfold find_ST in *.
+  apply lookup_union_Some_raw.
+  destruct (stty !! l) eqn:Hbase.
+  - left.
+    assert (Hbase_ext := Hbase).
+    apply Hext in Hbase_ext.
+    unfold find_ST in Hbase_ext.
+    rewrite Hfind in Hbase_ext.
+    inversion Hbase_ext; subst.
+    assumption.
+  - right. split; [exact Hbase |].
+    assert (Hdiff2 : (stty2 ∖ stty) !! l = Some t).
+    { apply lookup_difference_Some. split; auto. }
+    apply lookup_union_Some_raw.
+    right. split; [| assumption].
+    assert (Hdisj_spec : forall i x y,
+               (stty1 ∖ stty) !! i = Some x ->
+               (stty2 ∖ stty) !! i = Some y -> False)
+      by (apply map_disjoint_spec; assumption).
+    destruct ((stty1 ∖ stty) !! l) eqn:Hdiff1; auto.
+    exfalso. eapply Hdisj_spec; eauto.
+Qed.
+
+Lemma Phi_Heap_Step_preserves_updates :
+  forall phi phi' heap heap' k v,
+    (phi, heap) ===> (phi', heap') ->
+    Phi_Updates k v phi' ->
+    Phi_Updates k v phi.
+Proof.
+  intros phi phi' heap heap' k v HStep.
+  dependent induction HStep; intros HUpdate; inversion HUpdate; subst; eauto using Phi_Updates.
+Qed.
+
+Lemma Phi_Heap_StepsAux_preserves_updates :
+  forall phi heap phi' heap' n k v,
+    (phi, heap) =a=>* (phi', heap', n) ->
+    Phi_Updates k v phi' ->
+    Phi_Updates k v phi.
+Proof.
+  intros phi heap phi' heap' n k v HSteps.
+  dependent induction HSteps; intros HUpdate.
+  - assumption.
+  - eapply Phi_Heap_Step_preserves_updates; eauto.
+  - eapply IHHSteps1; try reflexivity.
+    eapply IHHSteps2; try reflexivity; eauto.
+Qed.
+
+Lemma Phi_Heap_Step_preserves_allocates :
+  forall phi phi' heap heap' k,
+    (phi, heap) ===> (phi', heap') ->
+    Phi_Allocates k phi' ->
+    Phi_Allocates k phi.
+Proof.
+  intros phi phi' heap heap' k HStep.
+  dependent induction HStep; intros HAlloc; inversion HAlloc; subst; eauto using Phi_Allocates.
+Qed.
+
+Lemma Phi_Heap_StepsAux_preserves_allocates :
+  forall phi heap phi' heap' n k,
+    (phi, heap) =a=>* (phi', heap', n) ->
+    Phi_Allocates k phi' ->
+    Phi_Allocates k phi.
+Proof.
+  intros phi heap phi' heap' n k HSteps.
+  dependent induction HSteps; intros HAlloc.
+  - assumption.
+  - eapply Phi_Heap_Step_preserves_allocates; eauto.
+  - eapply IHHSteps1; try reflexivity.
+    eapply IHHSteps2; try reflexivity; eauto.
+Qed.
+
+Lemma Phi_Heap_Step_lookup_source :
+  forall phi phi' heap heap' k v,
+    (phi, heap) ===> (phi', heap') ->
+    find_H k heap' = Some v ->
+    find_H k heap = Some v \/ Phi_Updates k v phi.
+Proof.
+  intros phi phi' heap heap' k v HStep.
+  dependent induction HStep; intros Hfind; simpl in *.
+  - destruct (decide (k = (r, l))) as [Heq | Hneq].
+    + subst.
+      assert (Hsame : find_H (r, l) (update_H ((r, l), v0) heap) = Some v0).
+      { unfold find_H, update_H. simpl. apply H_same_key_1. }
+      rewrite Hsame in Hfind. inversion Hfind; subst.
+      right. constructor.
+    + left. unfold find_H, update_H in Hfind. simpl in Hfind.
+      unfold find_H. eapply H_diff_keys_1; eauto.
+  - left. assumption.
+  - destruct (decide (k = (r, l))) as [Heq | Hneq].
+    + subst.
+      assert (Hsame : find_H (r, l) (update_H ((r, l), v0) heap) = Some v0).
+      { unfold find_H, update_H. simpl. apply H_same_key_1. }
+      rewrite Hsame in Hfind. inversion Hfind; subst.
+      right. constructor.
+    + left. unfold find_H, update_H in Hfind. simpl in Hfind.
+      unfold find_H. eapply H_diff_keys_1; eauto.
+  - destruct (IHHStep _ _ _ _ eq_refl eq_refl Hfind) as [HOld | HUpdate].
+    + left. assumption.
+    + right. now apply PU_Seq_L.
+  - destruct (IHHStep _ _ _ _ eq_refl eq_refl Hfind) as [HOld | HUpdate].
+    + left. assumption.
+    + right. now apply PU_Seq_R.
+  - left. assumption.
+  - destruct (IHHStep _ _ _ _ eq_refl eq_refl Hfind) as [HOld | HUpdate].
+    + left. assumption.
+    + right. now apply PU_Par_L.
+  - destruct (IHHStep _ _ _ _ eq_refl eq_refl Hfind) as [HOld | HUpdate].
+    + left. assumption.
+    + right. now apply PU_Par_R.
+  - left. assumption.
+Qed.
+
+Lemma Phi_Heap_StepsAux_lookup_source :
+  forall phi heap phi' heap' n k v,
+    (phi, heap) =a=>* (phi', heap', n) ->
+    find_H k heap' = Some v ->
+    find_H k heap = Some v \/ Phi_Updates k v phi.
+Proof.
+  intros phi heap phi' heap' n k v HSteps.
+  generalize dependent v.
+  generalize dependent k.
+  dependent induction HSteps; intros k v Hfind.
+  - left. assumption.
+  - eapply Phi_Heap_Step_lookup_source; eauto.
+  - destruct (IHHSteps2 _ _ _ _ _ eq_refl eq_refl k v Hfind) as [Hmid | HUpdateMid].
+    + destruct (IHHSteps1 _ _ _ _ _ eq_refl eq_refl k v Hmid) as [Hstart | HUpdateStart].
+      * left. assumption.
+      * right. assumption.
+    + right.
+      eapply Phi_Heap_StepsAux_preserves_updates; eauto.
+Qed.
+
+Lemma Phi_Heap_Steps_lookup_source :
+  forall phi heap phi' heap' k v,
+    (phi, heap) ==>* (phi', heap') ->
+    find_H k heap' = Some v ->
+    find_H k heap = Some v \/ Phi_Updates k v phi.
+Proof.
+  intros phi heap phi' heap' k v [n HSteps] Hfind.
+  eapply Phi_Heap_StepsAux_lookup_source; eauto.
+Qed.
+
+Lemma Phi_Heap_Step_preserves_domain :
+  forall phi phi' heap heap' k v,
+    (phi, heap) ===> (phi', heap') ->
+    find_H k heap = Some v ->
+    exists v', find_H k heap' = Some v'.
+Proof.
+  intros phi phi' heap heap' k v HStep.
+  dependent induction HStep; intros Hfind; simpl in *.
+  - destruct (decide (k = (r, l))).
+    + subst. exists v0. unfold find_H, update_H. simpl. apply H_same_key_1.
+    + exists v. unfold find_H in Hfind. unfold find_H, update_H. simpl.
+      eapply H_diff_keys_2; eauto.
+  - exists v. assumption.
+  - destruct (decide (k = (r, l))).
+    + subst. exists v0. unfold find_H, update_H. simpl. apply H_same_key_1.
+    + exists v. unfold find_H in Hfind. unfold find_H, update_H. simpl.
+      eapply H_diff_keys_2; eauto.
+  - eapply IHHStep; try reflexivity; eauto.
+  - eapply IHHStep; try reflexivity; eauto.
+  - exists v. assumption.
+  - eapply IHHStep; try reflexivity; eauto.
+  - eapply IHHStep; try reflexivity; eauto.
+  - exists v. assumption.
+Qed.
+
+Lemma Phi_Heap_StepsAux_preserves_domain :
+  forall phi heap phi' heap' n k v,
+    (phi, heap) =a=>* (phi', heap', n) ->
+    find_H k heap = Some v ->
+    exists v', find_H k heap' = Some v'.
+Proof.
+  intros phi heap phi' heap' n k v HSteps.
+  generalize dependent v.
+  generalize dependent k.
+  dependent induction HSteps; intros k v Hfind.
+  - exists v. assumption.
+  - eapply Phi_Heap_Step_preserves_domain; eauto.
+  - destruct (IHHSteps1 _ _ _ _ _ eq_refl eq_refl k v Hfind) as [vmid Hmid].
+    destruct (IHHSteps2 _ _ _ _ _ eq_refl eq_refl k vmid Hmid) as [vfinal Hfinal].
+    exists vfinal. assumption.
+Qed.
+
+Lemma Phi_Heap_Steps_preserves_domain :
+  forall phi heap phi' heap' k v,
+    (phi, heap) ==>* (phi', heap') ->
+    find_H k heap = Some v ->
+    exists v', find_H k heap' = Some v'.
+Proof.
+  intros phi heap phi' heap' k v [n HSteps] Hfind.
+  eapply Phi_Heap_StepsAux_preserves_domain; eauto.
+Qed.
+
+Lemma Phi_Heap_Step_alloc_source :
+  forall phi phi' heap heap' k v,
+    (phi, heap) ===> (phi', heap') ->
+    find_H k heap' = Some v ->
+    find_H k heap = None ->
+    Phi_Allocates k phi.
+Proof.
+  intros phi phi' heap heap' k v HStep.
+  dependent induction HStep; intros Hfind Hnone; simpl in *.
+  - destruct (decide (k = (r, l))) as [Heq | Hneq].
+    + subst. constructor.
+    + unfold find_H, update_H in Hfind. simpl in Hfind.
+      assert (Hold : find_H k heap = Some v).
+      { unfold find_H. eapply H_diff_keys_1; eauto. }
+      rewrite Hnone in Hold. discriminate.
+  - rewrite Hnone in Hfind. discriminate.
+  - destruct (decide (k = (r, l))) as [Heq | Hneq].
+    + subst. rewrite Hnone in H. contradiction.
+    + unfold find_H, update_H in Hfind. simpl in Hfind.
+      assert (Hold : find_H k heap = Some v).
+      { unfold find_H. eapply H_diff_keys_1; eauto. }
+      rewrite Hnone in Hold. discriminate.
+  - eauto using Phi_Allocates.
+  - eauto using Phi_Allocates.
+  - rewrite Hnone in Hfind. discriminate.
+  - eauto using Phi_Allocates.
+  - eauto using Phi_Allocates.
+  - rewrite Hnone in Hfind. discriminate.
+Qed.
+
+Lemma Phi_Heap_StepsAux_alloc_source :
+  forall phi heap phi' heap' n k v,
+    (phi, heap) =a=>* (phi', heap', n) ->
+    find_H k heap' = Some v ->
+    find_H k heap = None ->
+    Phi_Allocates k phi.
+Proof.
+  intros phi heap phi' heap' n k v HSteps.
+  generalize dependent v.
+  generalize dependent k.
+  dependent induction HSteps; intros k v Hfind Hnone.
+  - rewrite Hnone in Hfind. discriminate.
+  - eapply Phi_Heap_Step_alloc_source; eauto.
+  - destruct (find_H k heap'0) eqn:Hmid.
+    + eapply IHHSteps1; try reflexivity; eauto.
+    + assert (Halloc_mid : Phi_Allocates k phi'0).
+      { eapply IHHSteps2; try reflexivity; eauto. }
+      eapply Phi_Heap_StepsAux_preserves_allocates; eauto.
+Qed.
+
+Lemma Phi_Heap_Steps_alloc_source :
+  forall phi heap phi' heap' k v,
+    (phi, heap) ==>* (phi', heap') ->
+    find_H k heap' = Some v ->
+    find_H k heap = None ->
+    Phi_Allocates k phi.
+Proof.
+  intros phi heap phi' heap' k v [n HSteps] Hfind Hnone.
+  eapply Phi_Heap_StepsAux_alloc_source; eauto.
+Qed.
+
+Lemma Phi_Heap_Step_alloc_done :
+  forall phi phi' heap heap' k,
+    (phi, heap) ===> (phi', heap') ->
+    Phi_Allocates k phi \/ (exists v, find_H k heap = Some v) ->
+    Phi_Allocates k phi' \/ (exists v, find_H k heap' = Some v).
+Proof.
+  intros phi phi' heap heap' k HStep.
+  dependent induction HStep; intros HPending.
+  - destruct HPending as [HAlloc | [w Hfind]].
+    + inversion HAlloc; subst.
+      right. exists v. unfold find_H, update_H. simpl. apply H_same_key_1.
+    + right. eapply Phi_Heap_Step_preserves_domain with (v:=w);
+        [constructor; eauto | exact Hfind].
+  - destruct HPending as [HAlloc | [w Hfind]].
+    + inversion HAlloc.
+    + right. exists w. assumption.
+  - destruct HPending as [HAlloc | [w Hfind]].
+    + inversion HAlloc.
+    + right. eapply Phi_Heap_Step_preserves_domain with (v:=w);
+        [constructor; eauto | exact Hfind].
+  - destruct HPending as [HAlloc | [w Hfind]].
+    + inversion HAlloc; subst.
+      * destruct (IHHStep _ _ _ _ eq_refl eq_refl (or_introl H1)) as [HAlloc' | HDone].
+        -- left. now apply PA_Seq_L.
+        -- right. assumption.
+      * left. now apply PA_Seq_R.
+    + right. eapply Phi_Heap_Step_preserves_domain with (v:=w);
+        [constructor; eauto | exact Hfind].
+  - destruct HPending as [HAlloc | [w Hfind]].
+    + inversion HAlloc; subst.
+      * inversion H1.
+      * destruct (IHHStep _ _ _ _ eq_refl eq_refl (or_introl H1)) as [HAlloc' | HDone].
+        -- left. now apply PA_Seq_R.
+        -- right. assumption.
+    + right. eapply Phi_Heap_Step_preserves_domain with (v:=w);
+        [constructor; eauto | exact Hfind].
+  - destruct HPending as [HAlloc | [w Hfind]].
+    + inversion HAlloc; subst; inversion H1.
+    + right. exists w. assumption.
+  - destruct HPending as [HAlloc | [w Hfind]].
+    + inversion HAlloc; subst.
+      * destruct (IHHStep _ _ _ _ eq_refl eq_refl (or_introl H1)) as [HAlloc' | HDone].
+        -- left. now apply PA_Par_L.
+        -- right. assumption.
+      * left. now apply PA_Par_R.
+    + right. eapply Phi_Heap_Step_preserves_domain with (v:=w);
+        [constructor; eauto | exact Hfind].
+  - destruct HPending as [HAlloc | [w Hfind]].
+    + inversion HAlloc; subst.
+      * left. now apply PA_Par_L.
+      * destruct (IHHStep _ _ _ _ eq_refl eq_refl (or_introl H1)) as [HAlloc' | HDone].
+        -- left. now apply PA_Par_R.
+        -- right. assumption.
+    + right. eapply Phi_Heap_Step_preserves_domain with (v:=w);
+        [constructor; eauto | exact Hfind].
+  - destruct HPending as [HAlloc | [w Hfind]].
+    + inversion HAlloc; subst; inversion H1.
+    + right. exists w. assumption.
+  Unshelve. all: eauto.
+Qed.
+
+Lemma Phi_Heap_StepsAux_alloc_done :
+  forall phi heap phi' heap' n k,
+    (phi, heap) =a=>* (phi', heap', n) ->
+    Phi_Allocates k phi \/ (exists v, find_H k heap = Some v) ->
+    Phi_Allocates k phi' \/ (exists v, find_H k heap' = Some v).
+Proof.
+  intros phi heap phi' heap' n k HSteps.
+  dependent induction HSteps; intros HAlloc.
+  - assumption.
+  - eapply Phi_Heap_Step_alloc_done; eauto.
+  - eapply IHHSteps2; try reflexivity.
+    eapply IHHSteps1; try reflexivity; eauto.
+Qed.
+
+Lemma Phi_Heap_Steps_alloc_done :
+  forall phi heap heap' k,
+    (phi, heap) ==>* (Phi_Nil, heap') ->
+    Phi_Allocates k phi ->
+    exists v, find_H k heap' = Some v.
+Proof.
+  intros phi heap heap' k [n HSteps] HAlloc.
+  destruct (Phi_Heap_StepsAux_alloc_done phi heap Phi_Nil heap' n k HSteps
+              (or_introl HAlloc)) as [HNilAlloc | HDone].
+  - exfalso. eapply Phi_Allocates_nil_false; eauto.
+  - assumption.
+Qed.
   
 Lemma DisjointImpliesSomeOrNone:
   forall heap_1 heap_2,
@@ -218,13 +725,115 @@ Lemma TcHeap_Extended_2:
     (heap, env, rho, Mu_App ef1 ea1) ⇓ (heap_mu1, v1, acts_mu1) ->
     (heap, env, rho, Mu_App ef2 ea2) ⇓ (heap_mu2, v2, acts_mu2) ->
     (Phi_Par acts_mu1 acts_mu2, heap) ==>* (Phi_Nil, hp') ->
+    TcPhi stty1 acts_mu1 ->
+    TcPhi stty2 acts_mu2 ->
     TcVal (stty1, v1, subst_rho rho ty1) ->
     TcVal (stty2, v2, subst_rho rho ty2) ->
     TcHeap (heap, stty) ->
+    (forall l t, find_ST l stty = Some t -> find_ST l stty1 = Some t) ->
+    (forall l t, find_ST l stty = Some t -> find_ST l stty2 = Some t) ->
     TcHeap (heap_mu1, stty1) ->
     TcHeap (heap_mu2, stty2) ->
     TcHeap (hp', stty ∪ (stty1 ∖ stty ∪ stty2 ∖ stty)).
-Admitted.
+Proof.
+  intros heap env rho ef1 ef2 ea1 ea2 v1 v2 ty1 ty2 acts_mu1 acts_mu2
+    heap_mu1 heap_mu2 stty stty1 stty2 hp'
+    HheapDisj Hstep1 Hstep2 Hpar HTcPhi1 HTcPhi2 _ _
+    HTcHeap Hext1 Hext2 HTcHeap1 HTcHeap2.
+  assert (HsttyDisj : stty1 ∖ stty ##ₘ stty2 ∖ stty)
+    by (eapply djt_heap_implies_djt_stty; eauto).
+  assert (Hsteps1 : (acts_mu1, heap) ==>* (Phi_Nil, heap_mu1))
+    by (eapply BigStep_replays_trace; eauto).
+  assert (Hsteps2 : (acts_mu2, heap) ==>* (Phi_Nil, heap_mu2))
+    by (eapply BigStep_replays_trace; eauto).
+  constructor.
+  - intros k v HfindHp.
+    destruct (Phi_Heap_Steps_lookup_source
+                (Phi_Par acts_mu1 acts_mu2) heap Phi_Nil hp' k v Hpar HfindHp)
+      as [HfindBase | Hupdate].
+    + inversion HTcHeap as [? ? HHeapStore _ _]; subst.
+      destruct (HHeapStore k v HfindBase) as [t HfindStty].
+      exists t. eapply StoreTyping_Extended_Base; eauto.
+    + inversion Hupdate; subst.
+      * match goal with
+        | H : Phi_Updates k v acts_mu1 |- _ =>
+            destruct (HTcPhi1 k v H) as [t [HfindStty1 _]]
+        end.
+        exists t. eapply StoreTyping_Extended_Left; eauto.
+      * match goal with
+        | H : Phi_Updates k v acts_mu2 |- _ =>
+            destruct (HTcPhi2 k v H) as [t [HfindStty2 _]]
+        end.
+        exists t. eapply StoreTyping_Extended_Right; eauto.
+  - intros k t HfindStore.
+    unfold find_ST in HfindStore.
+    apply lookup_union_Some_raw in HfindStore.
+    destruct HfindStore as [HfindBaseStore | [HbaseNone HfindDiffs]].
+    + inversion HTcHeap as [? ? _ HStoreHeap _]; subst.
+      destruct (HStoreHeap k t HfindBaseStore) as [v HfindHeap].
+      eapply Phi_Heap_Steps_preserves_domain; eauto.
+    + apply lookup_union_Some_raw in HfindDiffs.
+      destruct HfindDiffs as [HfindDiff1 | [_ HfindDiff2]].
+      * apply lookup_difference_Some in HfindDiff1.
+        destruct HfindDiff1 as [HfindStty1 HfindBaseNone].
+        inversion HTcHeap1 as [? ? _ HStoreHeap1 _]; subst.
+        destruct (HStoreHeap1 k t HfindStty1) as [v HfindHeapMu1].
+        assert (HfindHeapNone : find_H k heap = None).
+        { eapply TcHeap_none_implies_none; eauto. }
+        assert (Halloc : Phi_Allocates k acts_mu1).
+        { eapply Phi_Heap_Steps_alloc_source; eauto. }
+        eapply Phi_Heap_Steps_alloc_done; eauto.
+        now apply PA_Par_L.
+      * apply lookup_difference_Some in HfindDiff2.
+        destruct HfindDiff2 as [HfindStty2 HfindBaseNone].
+        inversion HTcHeap2 as [? ? _ HStoreHeap2 _]; subst.
+        destruct (HStoreHeap2 k t HfindStty2) as [v HfindHeapMu2].
+        assert (HfindHeapNone : find_H k heap = None).
+        { eapply TcHeap_none_implies_none; eauto. }
+        assert (Halloc : Phi_Allocates k acts_mu2).
+        { eapply Phi_Heap_Steps_alloc_source; eauto. }
+        eapply Phi_Heap_Steps_alloc_done; eauto.
+        now apply PA_Par_R.
+  - intros k v t HfindHp HfindStore.
+    destruct (Phi_Heap_Steps_lookup_source
+                (Phi_Par acts_mu1 acts_mu2) heap Phi_Nil hp' k v Hpar HfindHp)
+      as [HfindBase | Hupdate].
+    + inversion HTcHeap as [? ? HHeapStore _ HHeapVals]; subst.
+      destruct (HHeapStore k v HfindBase) as [t0 HfindStty].
+      assert (HfindStore0 :
+                find_ST k (stty ∪ (stty1 ∖ stty ∪ stty2 ∖ stty)) = Some t0)
+        by (eapply StoreTyping_Extended_Base; eauto).
+      assert (t = t0)
+        by (eapply PairType_unique_type; eauto).
+      subst.
+      eapply ext_stores__val with (stty:=stty); eauto.
+      intros l t' Hfind. eapply StoreTyping_Extended_Base; eauto.
+    + inversion Hupdate; subst.
+      * match goal with
+        | H : Phi_Updates k v acts_mu1 |- _ =>
+            destruct (HTcPhi1 k v H) as [t1 [HfindStty1 HTcVal1]]
+        end.
+        assert (HfindStore1 :
+                  find_ST k (stty ∪ (stty1 ∖ stty ∪ stty2 ∖ stty)) = Some t1)
+          by (eapply StoreTyping_Extended_Left; eauto).
+        assert (t = t1)
+          by (eapply PairType_unique_type; eauto).
+        subst.
+        eapply ext_stores__val with (stty:=stty1); eauto.
+        intros l t' Hfind. eapply StoreTyping_Extended_Left; eauto.
+      * match goal with
+        | H : Phi_Updates k v acts_mu2 |- _ =>
+            destruct (HTcPhi2 k v H) as [t2 [HfindStty2 HTcVal2]]
+        end.
+        assert (HfindStore2 :
+                  find_ST k (stty ∪ (stty1 ∖ stty ∪ stty2 ∖ stty)) = Some t2)
+          by (eapply StoreTyping_Extended_Right; eauto).
+        assert (t = t2)
+          by (eapply PairType_unique_type; eauto).
+        subst.
+        eapply ext_stores__val with (stty:=stty2); eauto.
+        intros l t' Hfind. eapply StoreTyping_Extended_Right; eauto.
+Qed.
 
       
 Lemma subst_rho_eps_aux_1 :
@@ -233,7 +842,16 @@ Lemma subst_rho_eps_aux_1 :
    lc_type_sa sa' ->
    fold_subst_eps rho e1 = (fold_subst_eps rho' (closing_rgn_in_eps n x e)) ->
    fold_subst_sa rho sa = fold_subst_sa rho' (closing_rgn_in_sa n x sa') /\ e1 sa /\ e sa'.
-Admitted.
+Proof.
+  intros rho rho' n x e e1 sa sa' Hlc _ _.
+  exfalso.
+  inversion Hlc as [eps HAll]; subst.
+  destruct (HAll (SA_Alloc (Rgn_BVar true true 0))) as [_ HBad].
+  inversion HBad; subst.
+  match goal with
+  | H : lc_type_rgn (Rgn_BVar _ _ _) |- _ => inversion H
+  end.
+Qed.
 
 
 Lemma subst_rho_open_close_rgn :
@@ -263,7 +881,7 @@ Proof.
   - rewrite subst_rho_index in H. rewrite subst_rho_rgn_const in H. inversion H.
   - destruct (Ascii.ascii_dec r x); subst; simpl in *.
     + repeat rewrite subst_rho_index in H. inversion H; subst.
-      rewrite NPeano.Nat.eqb_refl.
+      rewrite Nat.eqb_refl.
       rewrite subst_rho_rgn_const.
       dependent induction w; simpl.
       * inversion HF; subst.
@@ -472,7 +1090,7 @@ Qed.
 
   
 
-Lemma ty_sound:
+Lemma ty_sound_strong:
   forall e env rho hp hp' v dynamic_eff,
     (hp, env, rho, e) ⇓ (hp', v, dynamic_eff) ->
     forall stty ctxt rgns t static_eff,
@@ -484,30 +1102,31 @@ Lemma ty_sound:
       exists stty',
         (forall l t', find_ST l stty = Some t' -> find_ST l stty' = Some t')
          /\ TcHeap (hp', stty')
-         /\ TcVal (stty', v, subst_rho rho t).
+         /\ TcVal (stty', v, subst_rho rho t)
+         /\ TcPhi stty' dynamic_eff.
 Proof.
   intros e env rho hp hp'  v dynamic_eff D. 
   dynamic_cases (dependent induction D) Case;
   intros stty ctxt rgns t static_eff Hhp Hrho Hinc Henv Hexp; 
   inversion Hexp; subst.    
   Case "cnt n"%string.
-    exists stty; (split; [| split]; auto). rewrite subst_rho_natural.
-    econstructor; eassumption.
+    exists stty; split; [auto |]; split; [auto |]; split;
+      [try rewrite subst_rho_natural; apply TC_Num | apply TcPhi_nil].
   Case "bool b".
-    exists stty;  (split; [| split]; auto). rewrite subst_rho_boolean.
-    econstructor; eassumption. 
+    exists stty; split; [auto |]; split; [auto |]; split;
+      [try rewrite subst_rho_boolean; apply TC_Bit | apply TcPhi_nil].
   Case "var x".
-    exists stty; (split; [| split]; auto).
-    eapply ty_sound_var; eassumption. 
+    exists stty; split; [auto |]; split; [auto |]; split;
+      [eapply ty_sound_var; eassumption | apply TcPhi_nil].
   Case "mu_abs".
-    exists stty; (split; [| split]; auto). 
-    eapply ty_sound_closure; try (solve [eassumption]). auto.
+    exists stty; split; [auto |]; split; [auto |]; split;
+      [eapply ty_sound_closure; try (solve [eassumption]); auto | apply TcPhi_nil].
   Case "rgn_abs".
-    exists stty;  (split; [| split]; auto).  
-    eapply ty_sound_region_closure; try (solve [eassumption]).
+    exists stty; split; [auto |]; split; [auto |]; split;
+      [eapply ty_sound_region_closure; try (solve [eassumption]) | apply TcPhi_nil].
   Case "mu_app".
-    edestruct IHD1 as [sttym [Weak1 [TcHeap1 TcVal_mu]]]; eauto. 
-    edestruct IHD2 as [sttya [Weaka [TcHeapa TcVal_arg]]]; eauto.  
+    edestruct IHD1 as [sttym [Weak1 [TcHeap1 [TcVal_mu TcPhi_mu]]]]; eauto. 
+    edestruct IHD2 as [sttya [Weaka [TcHeapa [TcVal_arg TcPhi_arg]]]]; eauto.  
     eapply ext_stores__env; eauto.
     inversion TcVal_mu as [ | | | ? ? ? ? ? ? ? TcRho_rho' TcRho_Inc' TcEnv_env' TcExp_abs | | |] ; subst.    
     inversion TcExp_abs as [ | |  | ? ? ? ? ? ? ? ? ? ? ? ? ? TcExp_ec TcExp_ee | | | | | | | | | | | | | | | | | | | | | ]; subst.   
@@ -519,7 +1138,7 @@ Proof.
     unfold update_rec_E, update_rec_T in *.     
     edestruct IHD3 with (ctxt:=update_T (x, tyx)
                                  (update_T (f, Ty_Arrow tyx effc0 tyc effe0 Ty_Effect) ctxt0))
-      as [sttyb [Weakb [TcHeapb TcVal_res]]]; eauto. simpl in *.
+      as [sttyb [Weakb [TcHeapb [TcVal_res TcPhi_res]]]]; eauto. simpl in *.
     SCase "TcInc".
     {apply ExtendedTcInv_2. 
      - assumption.
@@ -531,36 +1150,53 @@ Proof.
       apply update_env. apply update_env. eapply ext_stores__env; eauto.  
       eapply ext_stores__val; eauto. eassumption.
     SCase "TcHeap".
-      exists sttyb; intuition.  
+      exists sttyb. split.
+      { intros l t' Hfind. apply Weakb. apply Weaka. now apply Weak1. }
+      split; [assumption |].
+      split; [assumption |].
+      assert (HTcPhi_fun_arg : TcPhi sttyb (Phi_Seq facts aacts)).
+      { apply TcPhi_seq;
+        [ eapply TcPhi_weaken with (stty:=sttym);
+          [intros l t' Hfind; apply Weakb; now apply Weaka | exact TcPhi_mu]
+        | eapply TcPhi_weaken with (stty:=sttya);
+          [exact Weakb | exact TcPhi_arg] ]. }
+      apply TcPhi_seq; assumption.
     SCase "TcVal".
-      edestruct IHD1 as [sttyl [Weak1 [TcHeap1 TcVal_lam]]]; eauto. 
+      edestruct IHD1 as [sttyl [Weak1 [TcHeap1 [TcVal_lam TcPhi_lam]]]]; eauto. 
       inversion TcVal_lam as  [ | | | ? ? ? ? ? ? ?  TcRho_rho' TcInc'  TcEnv_env' TcExp_lam | | |]; subst.   
       inversion TcExp_lam as [ | | | | ? ? ? ? ? ? ? ? ? TcExp_eb | | | | | | | | | | | | | | | | | | | |  ]; subst.   
       { edestruct IHD2 with (rgns:=set_union rgns0 (singleton_set x))
-        as [sttyr [Weak2 [TcHeap2 TcVal_res]]]; eauto using update_env, ext_stores__env.
+        as [sttyr [Weak2 [TcHeap2 [TcVal_res TcPhi_res]]]]; eauto using update_env, ext_stores__env.
         - { apply update_rho; [ assumption | assumption]. }
         - apply update_inc. assumption.
         - eapply extended_rho; eauto.
-        - exists sttyr; intuition. 
-          rewrite subst_rho_forallrgn in H5.
-          rewrite subst_rho_forallrgn in H5.
-          inversion H5.  
-          unfold update_R in TcVal_res. 
-          simpl in TcVal_res. rewrite subst_add_comm in TcVal_res.
-          + unfold subst_in_type in TcVal_res.
-            rewrite SUBST_AS_CLOSE_OPEN in TcVal_res; auto.
-            erewrite subst_rho_open_close in TcVal_res; eauto.
-          + eapply map_to_list_unique with (m:=<[x:=v']> rho'); eauto.
-          + apply not_elem_of_dom.
-            eapply bound_var_is_fresh; eauto. }
+        - exists sttyr. split.
+          { intros l t' Hfind. apply Weak2. now apply Weak1. }
+          split; [assumption |].
+          split.
+          + rewrite subst_rho_forallrgn in H5.
+            rewrite subst_rho_forallrgn in H5.
+            inversion H5.  
+            unfold update_R in TcVal_res. 
+            simpl in TcVal_res. rewrite subst_add_comm in TcVal_res.
+            * unfold subst_in_type in TcVal_res.
+              rewrite SUBST_AS_CLOSE_OPEN in TcVal_res; auto.
+              erewrite subst_rho_open_close in TcVal_res; eauto.
+            * eapply map_to_list_unique with (m:=<[x:=v']> rho'); eauto.
+            * apply not_elem_of_dom.
+              eapply bound_var_is_fresh; eauto.
+          + apply TcPhi_seq.
+            * eapply TcPhi_weaken with (stty:=sttyl);
+                [exact Weak2 | exact TcPhi_lam].
+            * exact TcPhi_res. }
   Case "eff_app". 
-    edestruct IHD1 as [sttym [Weak1 [TcHeap1 TcVal_mu]]]; eauto.
-    edestruct IHD2 as [sttya [Weaka [TcHeapa TcVal_arg]]]; eauto using ext_stores__env.
+    edestruct IHD1 as [sttym [Weak1 [TcHeap1 [TcVal_mu TcPhi_mu]]]]; eauto.
+    edestruct IHD2 as [sttya [Weaka [TcHeapa [TcVal_arg TcPhi_arg]]]]; eauto using ext_stores__env.
     inversion TcVal_mu as  [ | | | ? ? ? ? ? ? ? TcRho_rho' TcInc' TcEnv_env' TcExp_abs | | |]; subst. 
     inversion TcExp_abs as [ | | | | ? ? ? ? ? ? ? ? ? TcExp_eb | | | | | | | | | | | | | | | | | | | |  ]; subst. 
     edestruct IHD3 with (ctxt:=update_T (x, tyx)
                                  (update_T (f, Ty_Arrow tyx effc0 tyc0 effe0 Ty_Effect) ctxt0))
-      as [sttyb [Weakb [TcHeapb TcVal_res]]]; eauto. simpl in *.
+      as [sttyb [Weakb [TcHeapb [TcVal_res TcPhi_res]]]]; eauto. simpl in *.
     SCase "Extended Inc". 
     {apply ExtendedTcInv_2. 
      - assumption.
@@ -579,41 +1215,60 @@ Proof.
         inversion H4. 
         assert (SubstEq: subst_rho rho' tyx = subst_rho rho tya) by assumption.
         rewrite <- SubstEq in TcVal_arg.  eassumption. 
-        exists sttyb. intuition.
-    rewrite subst_rho_effect. rewrite subst_rho_effect in TcVal_res.
-    assumption.
+        exists sttyb. split.
+        { intros l t' Hfind. apply Weakb. apply Weaka. now apply Weak1. }
+        split; [assumption |].
+        split.
+        { rewrite subst_rho_effect. rewrite subst_rho_effect in TcVal_res.
+          assumption. }
+        assert (HTcPhi_fun_arg : TcPhi sttyb (Phi_Seq facts aacts)).
+        { apply TcPhi_seq;
+          [ eapply TcPhi_weaken with (stty:=sttym);
+            [intros l t' Hfind; apply Weakb; now apply Weaka | exact TcPhi_mu]
+          | eapply TcPhi_weaken with (stty:=sttya);
+            [exact Weakb | exact TcPhi_arg] ]. }
+        apply TcPhi_seq; assumption.
   Case "par_pair".
-    edestruct IHD3 as [sttym [Weak1 [TcHeap1 TcVal_app1]]]; eauto.  
-    edestruct IHD4 as [sttya [Weaka [TcHeapa TcVal_app2]]]; eauto. 
+    edestruct IHD3 as [sttym [Weak1 [TcHeap1 [TcVal_app1 TcPhi_app1]]]]; eauto.  
+    edestruct IHD4 as [sttya [Weaka [TcHeapa [TcVal_app2 TcPhi_app2]]]]; eauto. 
     assert (exists stty' : Sigma,
            (forall (l : SigmaKey) (t' : Tau),
             find_ST l stty = Some t' -> find_ST l stty' = Some t') /\
-             TcHeap (heap_eff1, stty') /\ TcVal (stty', Eff theta1, subst_rho rho ty3))
+             TcHeap (heap_eff1, stty') /\
+             TcVal (stty', Eff theta1, subst_rho rho ty3) /\
+             TcPhi stty' acts_eff1)
       as HTyped3.
     eapply IHD1; eauto.
     assert (exists stty' : Sigma,
            (forall (l : SigmaKey) (t' : Tau),
             find_ST l stty = Some t' -> find_ST l stty' = Some t') /\
-             TcHeap (heap_eff2, stty') /\ TcVal (stty', Eff theta2, subst_rho rho ty4))
+             TcHeap (heap_eff2, stty') /\
+             TcVal (stty', Eff theta2, subst_rho rho ty4) /\
+             TcPhi stty' acts_eff2)
       as HTyped4.
     eapply IHD2; eauto.
     assert (exists stty' : Sigma,
            (forall (l : SigmaKey) (t' : Tau),
             find_ST l stty = Some t' -> find_ST l stty' = Some t') /\
-             TcHeap (heap_mu1, stty') /\ TcVal (stty', v1, subst_rho rho ty1))
+             TcHeap (heap_mu1, stty') /\
+             TcVal (stty', v1, subst_rho rho ty1) /\
+             TcPhi stty' acts_mu1)
       as HTyped1.
     eapply IHD3; eauto.
     assert (exists stty' : Sigma,
            (forall (l : SigmaKey) (t' : Tau),
             find_ST l stty = Some t' -> find_ST l stty' = Some t') /\
-             TcHeap (heap_mu2, stty') /\ TcVal (stty', v2, subst_rho rho ty2))
+             TcHeap (heap_mu2, stty') /\
+             TcVal (stty', v2, subst_rho rho ty2) /\
+             TcPhi stty' acts_mu2)
       as HTyped2.
     eapply IHD4; eauto.
-    destruct HTyped1 as[ stty1 [HA1  [HA2 HA3]]].
-    destruct HTyped2 as[ stty2 [HB1  [HB2 HB3]]].
-    destruct HTyped3 as[ stty3 [HC1  [HC2 HC3]]].
-    destruct HTyped4 as[ stty4 [HD1  [HD2 HD3]]].  
+    destruct HTyped1 as[ stty1 [HA1  [HA2 [HA3 HA4]]]].
+    destruct HTyped2 as[ stty2 [HB1  [HB2 [HB3 HB4]]]].
+    destruct HTyped3 as[ stty3 [HC1  [HC2 [HC3 HC4]]]].
+    destruct HTyped4 as[ stty4 [HD1  [HD2 [HD3 HD4]]]].  
     { exists (stty ∪ ((stty1 ∖ stty) ∪ (stty2 ∖ stty))).
+      destruct H0 as [HEff1 HEff2].
       split.  
       + assert (stty1 ∖ stty ##ₘ stty2 ∖ stty)
           by (eapply djt_heap_implies_djt_stty; eauto).
@@ -622,65 +1277,120 @@ Proof.
         assert (find_ST l stty2 = Some t') by (apply HB1; auto).
         intros. eapply StoreTyping_Union_2; eauto.
       + split.
-        * eapply TcHeap_Extended_2
-            with (acts_mu1:=acts_mu1) (acts_mu2:=acts_mu2); eauto.
-        * eapply TcValExtended_2; eauto.
-          eapply djt_heap_implies_djt_stty; eauto.
+          * eapply TcHeap_Extended_2
+              with (acts_mu1:=acts_mu1) (acts_mu2:=acts_mu2); eauto.
+        * split.
+          -- eapply TcValExtended_2; eauto.
+             eapply djt_heap_implies_djt_stty; eauto.
+          -- assert (HsttyDisj : stty1 ∖ stty ##ₘ stty2 ∖ stty)
+               by (eapply djt_heap_implies_djt_stty; eauto).
+             assert (HCto :
+                       forall l t',
+                         find_ST l stty3 = Some t' ->
+                         find_ST l (stty ∪ (stty1 ∖ stty ∪ stty2 ∖ stty)) = Some t').
+             { intros l t' Hfind3.
+               inversion HC2 as [? ? _ HStoreHeap3 _]; subst.
+               destruct (HStoreHeap3 l t' Hfind3) as [v HfindEff].
+               unfold equiv, heap_equiv in HEff1; subst heap_eff1.
+               inversion Hhp as [? ? HHeapStore _ _]; subst.
+               destruct (HHeapStore l v HfindEff) as [t0 HfindBase].
+               assert (Hfind3base : find_ST l stty3 = Some t0)
+                 by (apply HC1; assumption).
+               assert (t' = t0) by (eapply PairType_unique_type; eauto).
+               subst. eapply StoreTyping_Extended_Base; eauto. }
+             assert (HDto :
+                       forall l t',
+                         find_ST l stty4 = Some t' ->
+                         find_ST l (stty ∪ (stty1 ∖ stty ∪ stty2 ∖ stty)) = Some t').
+             { intros l t' Hfind4.
+               inversion HD2 as [? ? _ HStoreHeap4 _]; subst.
+               destruct (HStoreHeap4 l t' Hfind4) as [v HfindEff].
+               unfold equiv, heap_equiv in HEff2; subst heap_eff2.
+               inversion Hhp as [? ? HHeapStore _ _]; subst.
+               destruct (HHeapStore l v HfindEff) as [t0 HfindBase].
+               assert (Hfind4base : find_ST l stty4 = Some t0)
+                 by (apply HD1; assumption).
+               assert (t' = t0) by (eapply PairType_unique_type; eauto).
+               subst. eapply StoreTyping_Extended_Base; eauto. }
+             assert (HTcPhi_eff :
+                       TcPhi (stty ∪ (stty1 ∖ stty ∪ stty2 ∖ stty))
+                         (Phi_Par acts_eff1 acts_eff2)).
+             { apply TcPhi_par.
+               - eapply TcPhi_weaken with (stty:=stty3); eauto.
+               - eapply TcPhi_weaken with (stty:=stty4); eauto. }
+             assert (HTcPhi_mu :
+                       TcPhi (stty ∪ (stty1 ∖ stty ∪ stty2 ∖ stty))
+                         (Phi_Par acts_mu1 acts_mu2)).
+             { apply TcPhi_par.
+               - eapply TcPhi_weaken with (stty:=stty1); eauto.
+                 intros l t' Hfind. eapply StoreTyping_Extended_Left; eauto.
+               - eapply TcPhi_weaken with (stty:=stty2); eauto.
+                 intros l t' Hfind. eapply StoreTyping_Extended_Right; eauto. }
+             apply TcPhi_seq; assumption.
     }
   Case "cond_true".
-    edestruct IHD1 as [sttyb [Weakb [TcHeapvb TcVal_e0]]]; eauto. 
-    edestruct IHD2 as [stty1 [Weak1 [TcHeapv1 TcVal_e1]]]; 
+    edestruct IHD1 as [sttyb [Weakb [TcHeapvb [TcVal_e0 TcPhi_e0]]]]; eauto. 
+    edestruct IHD2 as [stty1 [Weak1 [TcHeapv1 [TcVal_e1 TcPhi_e1]]]]; 
       eauto using ext_stores__env.
-    exists stty1. intuition.
+    exists stty1. split.
+    { intros l t' Hfind. apply Weak1. now apply Weakb. }
+    split; [assumption |].
+    split; [assumption |].
+    apply TcPhi_seq; [eapply TcPhi_weaken; eauto | assumption].
   Case "cond_false".
-    edestruct IHD1 as [sttyb [Weakb [TcHeapvb TcVal_e0]]]; eauto. 
-    edestruct IHD2 as [stty2 [Weak2 [TcHeapv2 TcVal_e2]]]; 
+    edestruct IHD1 as [sttyb [Weakb [TcHeapvb [TcVal_e0 TcPhi_e0]]]]; eauto. 
+    edestruct IHD2 as [stty2 [Weak2 [TcHeapv2 [TcVal_e2 TcPhi_e2]]]]; 
       eauto using ext_stores__env.
-    exists stty2. intuition.  
+    exists stty2. split.
+    { intros l t' Hfind. apply Weak2. now apply Weakb. }
+    split; [assumption |].
+    split; [assumption |].
+    apply TcPhi_seq; [eapply TcPhi_weaken; eauto | assumption].
   Case "new_ref e".
     edestruct IHD with (stty := stty)
                       (ctxt := ctxt)
                       (rgns := rgns)  
                       (t := t0)
                       (static_eff := veff)
-      as [sttyv [Weakv [TcHeapv TcVal_v]]]; eauto.
+      as [sttyv [Weakv [TcHeapv [TcVal_v TcPhi_v]]]]; eauto.
     assert (find_H (r, allocate_H heap' r) heap' = None)
       by (apply allocate_H_fresh).
-    exists (update_ST (r, allocate_H heap' r) (subst_rho rho t0) sttyv); split; [ | split].  
+    assert (HfreshST : find_ST (r, allocate_H heap' r) sttyv = None).
+    { destruct (find_ST (r, allocate_H heap' r) sttyv) as [t |] eqn:Hfind; auto.
+      inversion_clear TcHeapv as [? ? ? STfind_Hfind ?].
+      destruct (STfind_Hfind (r, allocate_H heap' r) t Hfind) as [? ex].
+      rewrite H0 in ex. discriminate. }
+    assert (Weakv_update :
+              forall k' t',
+                find_ST k' sttyv = Some t' ->
+                find_ST k'
+                  (update_ST (r, allocate_H heap' r)
+                     (subst_rho rho t0) sttyv) = Some t').
+    { intros k' t' STfind.
+      destruct (decide (k' = (r, allocate_H heap' r))) as [Heq | Hneq].
+      - subst. rewrite HfreshST in STfind. discriminate.
+      - apply G_diff_keys_2;
+          [ intro Heq; apply Hneq; now symmetry | assumption ]. }
+    exists (update_ST (r, allocate_H heap' r) (subst_rho rho t0) sttyv);
+      split; [ | split; [ | split]].
     SCase "Extended stores".
-      intros k' t' STfind. destruct k' as [r' l']. 
-      destruct (eq_nat_dec r r'); destruct (eq_nat_dec (allocate_H heap' r) l'); subst. 
-      SSCase "New address must be fresh, prove by contradiction".
-        apply Weakv in STfind. 
-        inversion_clear TcHeapv as [? ? ?  STfind_Hfind ?].  
-        destruct (STfind_Hfind (r', allocate_H heap' r') t' STfind) as [x F].
-        assert (C : None = Some x) by (rewrite <- F; rewrite <- H0; reflexivity).
-        discriminate. 
-      SSCase "Existing addresses are well-typed 1".
-        apply G_diff_keys_2; [ simpl; intuition; apply n; congruence |
-                             now apply Weakv in STfind ].
-      SSCase "Existing addresses are well-typed 2".
-        apply G_diff_keys_2; [ simpl; intuition; apply n; congruence |
-                           now apply Weakv in STfind ].
-      SSCase "Existing addresses are well-typed 3".
-         apply G_diff_keys_2; [simpl; intuition; apply n; congruence |
-                             now apply Weakv ].
+      intros k' t' STfind. apply Weakv_update. now apply Weakv.
     SCase "Heap typeness".
-      apply H_update_heap_fresh; eauto. 
-      remember (find_ST (r, allocate_H heap' r) sttyv) as to; symmetry in Heqto.
-      destruct to as [ t | ]. 
-      SSCase "New address must be fresh, prove by contradiction".
-        inversion_clear TcHeapv as [? ? ? STfind_Hfind ?].  
-        destruct (STfind_Hfind (r, allocate_H heap' r) t Heqto) as [? ex].
-        rewrite H0 in ex. discriminate.
-      SSCase "Heap typeness is preserved".
-        reflexivity. 
+      apply H_update_heap_fresh; eauto.
     SCase "Loc is well-typed".
       simpl in H; inversion H; subst. 
       rewrite subst_rho_tyref. unfold mk_rgn_type. rewrite subst_rho_rgn_const.
-      econstructor. apply lookup_insert.
-      intro.
-      eapply TcVal_implies_closed in TcVal_v; eauto.
+      econstructor;
+        [ unfold find_ST, update_ST; apply lookup_insert
+        | intro; eapply TcVal_implies_closed in TcVal_v; eauto ].
+    SCase "Trace is well-typed".
+      apply TcPhi_seq;
+        [ eapply TcPhi_weaken; eauto
+        | unfold TcPhi; intros k' v' HUpdate;
+          inversion HUpdate; subst;
+          exists (subst_rho rho t0); split;
+          [ unfold find_ST, update_ST; apply lookup_insert
+          | eapply ext_stores__val; eauto ] ].
   Case "get_ref e".
     edestruct IHD with (hp' := hp')
                       (v := Loc (Rgn_Const true false s) l) 
@@ -690,8 +1400,8 @@ Proof.
                       (t := Ty_Ref (mk_rgn_type ((Rgn_Const true false s))) t)
                       (static_eff := aeff)
                       (dynamic_eff := aacts)
-    as [sttyv [Weakv [TcHeapv TcVal_v]]]; eauto.
-    exists sttyv. split; [ | split].
+    as [sttyv [Weakv [TcHeapv [TcVal_v TcPhi_v]]]]; eauto.
+    exists sttyv. split; [ | split; [ | split]].
     SCase "HeapTyping extends".
       apply Weakv.
     SCase "Heap is well typed".
@@ -701,6 +1411,10 @@ Proof.
       inversion TcVal_v; subst; simpl in H; inversion H; subst.
       rewrite subst_rho_tyref in H7. inversion H7. subst.
       assumption.
+    SCase "Trace is well-typed".
+      apply TcPhi_seq;
+        [ assumption
+        | unfold TcPhi; intros k' v' HUpdate; inversion HUpdate ].
   Case "set_ref e1 e2".
     edestruct IHD1 with (hp' := heap')
                        (v := Loc (Rgn_Const true false s) l) 
@@ -710,68 +1424,147 @@ Proof.
                        (t := Ty_Ref (mk_rgn_type ((Rgn_Const true false s))) t0)
                        (static_eff := aeff)
                        (dynamic_eff := aacts)
-       as [sttya [Weaka [TcHeapa TcVal_a]]]; eauto.
+       as [sttya [Weaka [TcHeapa [TcVal_a TcPhi_a]]]]; eauto.
     edestruct IHD2 with (stty := sttya)
                        (ctxt := ctxt)
                        (rgns := rgns)  
                        (t := t0)
                        (static_eff := veff)
-      as [sttyv [Weakv [TcHeapv TcVal_v]]]; eauto using ext_stores__env.
-    exists sttyv. split; [ | split].
+      as [sttyv [Weakv [TcHeapv [TcVal_v TcPhi_v]]]]; eauto using ext_stores__env.
+    assert (HwriteST : find_ST (r, l) sttyv = Some (subst_rho rho t0)).
+    { apply Weakv. inversion TcVal_a; subst.
+      simpl in H0; inversion H0; subst.
+      match goal with
+      | Hty : _ = subst_rho _ (Ty_Ref _ _) |- _ =>
+          rewrite subst_rho_tyref in Hty; inversion Hty; subst
+      | Hty : subst_rho _ (Ty_Ref _ _) = _ |- _ =>
+          rewrite subst_rho_tyref in Hty; inversion Hty; subst
+      end.
+      assumption. }
+    exists sttyv. split; [ | split; [ | split]].
     SCase "HeapTyping extends".
       eapply weakening_trans; eauto.
     SCase "New heap is well typed".
       apply H_update_heap_exists with (t:= subst_rho rho t0).   
       { assumption. }
-      { apply Weakv. inversion TcVal_a; subst.  
-        simpl in H0; inversion H0; subst.
-        rewrite subst_rho_tyref in H5. inversion H5. subst.
-        assumption. }
+      { assumption. }
       { assumption. }
     SCase "Result value is well-typed".
       rewrite subst_rho_unit. constructor.
+    SCase "Trace is well-typed".
+      assert (HTcPhi_av : TcPhi sttyv (Phi_Seq aacts vacts)).
+      { apply TcPhi_seq;
+          [ eapply TcPhi_weaken with (stty:=sttya); eauto
+          | exact TcPhi_v ]. }
+      apply TcPhi_seq;
+        [ exact HTcPhi_av
+        | unfold TcPhi; intros k' v' HUpdate; inversion HUpdate; subst;
+          exists (subst_rho rho t0); split; [ exact HwriteST | exact TcVal_v ] ].
   Case "nat_plus x y".
-    edestruct IHD1 as [sttyx [Weakx [TcHeapvx TcVal_x]]]; eauto. 
-    edestruct IHD2 as [sttyy [Weaky [TcHeapvy TcVal_y]]]; 
+    edestruct IHD1 as [sttyx [Weakx [TcHeapvx [TcVal_x TcPhi_x]]]]; eauto. 
+    edestruct IHD2 as [sttyy [Weaky [TcHeapvy [TcVal_y TcPhi_y]]]]; 
       eauto using ext_stores__env. 
-    exists sttyy. intuition. rewrite subst_rho_natural. constructor.
+    exists sttyy. split.
+    { intros l t' Hfind. apply Weaky. now apply Weakx. }
+    split; [assumption |].
+    split; [rewrite subst_rho_natural; constructor |].
+    apply TcPhi_seq;
+      [ eapply TcPhi_weaken with (stty:=sttyx); eauto
+      | assumption ].
   Case "nat_minus x y".
-    edestruct IHD1 as [sttyx [Weakx [TcHeapvx TcVal_x]]]; eauto. 
-    edestruct IHD2 as [sttyy [Weaky [TcHeapvy TcVal_y]]]; 
+    edestruct IHD1 as [sttyx [Weakx [TcHeapvx [TcVal_x TcPhi_x]]]]; eauto. 
+    edestruct IHD2 as [sttyy [Weaky [TcHeapvy [TcVal_y TcPhi_y]]]]; 
       eauto using ext_stores__env.
-    exists sttyy. intuition. rewrite subst_rho_natural. constructor.
+    exists sttyy. split.
+    { intros l t' Hfind. apply Weaky. now apply Weakx. }
+    split; [assumption |].
+    split; [rewrite subst_rho_natural; constructor |].
+    apply TcPhi_seq;
+      [ eapply TcPhi_weaken with (stty:=sttyx); eauto
+      | assumption ].
   Case "nat_times x y".
-    edestruct IHD1 as [sttyx [Weakx [TcHeapvx TcVal_x]]]; eauto. 
-    edestruct IHD2 as [sttyy [Weaky [TcHeapvy TcVal_y]]]; 
+    edestruct IHD1 as [sttyx [Weakx [TcHeapvx [TcVal_x TcPhi_x]]]]; eauto. 
+    edestruct IHD2 as [sttyy [Weaky [TcHeapvy [TcVal_y TcPhi_y]]]]; 
       eauto using ext_stores__env.
-    exists sttyy. intuition. rewrite subst_rho_natural. constructor.
+    exists sttyy. split.
+    { intros l t' Hfind. apply Weaky. now apply Weakx. }
+    split; [assumption |].
+    split; [rewrite subst_rho_natural; constructor |].
+    apply TcPhi_seq;
+      [ eapply TcPhi_weaken with (stty:=sttyx); eauto
+      | assumption ].
   Case "bool_eq x y".
-    edestruct IHD1 as [sttyx [Weakx [TcHeapvx TcVal_x]]]; eauto. 
-    edestruct IHD2 as [sttyy [Weaky [TcHeapvy TcVal_y]]]; 
+    edestruct IHD1 as [sttyx [Weakx [TcHeapvx [TcVal_x TcPhi_x]]]]; eauto. 
+    edestruct IHD2 as [sttyy [Weaky [TcHeapvy [TcVal_y TcPhi_y]]]]; 
       eauto using ext_stores__env.
-    exists sttyy. intuition. rewrite subst_rho_boolean. constructor.
+    exists sttyy. split.
+    { intros l t' Hfind. apply Weaky. now apply Weakx. }
+    split; [assumption |].
+    split; [rewrite subst_rho_boolean; constructor |].
+    apply TcPhi_seq;
+      [ eapply TcPhi_weaken with (stty:=sttyx); eauto
+      | assumption ].
   Case "alloc_abs".
-    exists stty. intuition. rewrite subst_rho_effect. constructor.
+    exists stty; split; [auto |]; split; [auto |]; split;
+      [rewrite subst_rho_effect; constructor | subst; apply TcPhi_nil].
   Case "read_abs".
-    exists stty. intuition. rewrite subst_rho_effect. constructor.
+    exists stty; split; [auto |]; split; [auto |]; split;
+      [rewrite subst_rho_effect; constructor | subst; apply TcPhi_nil].
   Case "write_abs".
-    exists stty. intuition. rewrite subst_rho_effect. constructor.
+    exists stty; split; [auto |]; split; [auto |]; split;
+      [rewrite subst_rho_effect; constructor | subst; apply TcPhi_nil].
   Case "read_conc".
-    exists stty. intuition.
-    assert (hp = hp') by (eapply EmptyTracePreservesHeap_1; eauto; reflexivity); now subst.
-    rewrite subst_rho_effect. constructor.      
+    exists stty. split; [auto |].
+    split.
+    { assert (hp = hp') by (eapply EmptyTracePreservesHeap_1; eauto; reflexivity);
+      now subst. }
+    split; [rewrite subst_rho_effect; constructor | subst; apply TcPhi_nil].
   Case "write_conc".
-    exists stty. intuition.
-    assert (hp = hp') by (eapply EmptyTracePreservesHeap_1; eauto; reflexivity); now subst.
-    rewrite subst_rho_effect. constructor. 
+    exists stty. split; [auto |].
+    split.
+    { assert (hp = hp') by (eapply EmptyTracePreservesHeap_1; eauto; reflexivity);
+      now subst. }
+    split; [rewrite subst_rho_effect; constructor | subst; apply TcPhi_nil].
   Case "eff_concat".
-    exists stty. intuition. rewrite subst_rho_effect. constructor.
+    edestruct IHD1 as [sttya [Weaka [TcHeapa [TcVal_a TcPhi_a]]]]; eauto.
+    edestruct IHD2 with (stty := sttya)
+      as [sttyb [Weakb [TcHeapb [TcVal_b TcPhi_b]]]];
+      eauto using ext_stores__env.
+    exists sttyb. split.
+    { intros l t' Hfind. apply Weakb. now apply Weaka. }
+    split; [assumption |].
+    split; [rewrite subst_rho_effect; constructor |].
+    apply TcPhi_seq;
+      [ eapply TcPhi_weaken with (stty:=sttya); eauto
+      | assumption ].
   Case "eff_top".
-    exists stty. intuition. rewrite subst_rho_effect. constructor.
+    exists stty; split; [auto |]; split; [auto |]; split;
+      [rewrite subst_rho_effect; constructor | subst; apply TcPhi_nil].
   Case "eff_empty".
-    exists stty. intuition. rewrite subst_rho_effect. constructor.
-Admitted.
+    exists stty; split; [auto |]; split; [auto |]; split;
+      [rewrite subst_rho_effect; constructor | subst; apply TcPhi_nil].
+Qed.
+
+Lemma ty_sound:
+  forall e env rho hp hp' v dynamic_eff,
+    (hp, env, rho, e) ⇓ (hp', v, dynamic_eff) ->
+    forall stty ctxt rgns t static_eff,
+      TcHeap (hp, stty) ->
+      TcRho (rho, rgns) ->
+      TcInc (ctxt, rgns)->
+      TcEnv (stty, rho, env, ctxt) ->
+      TcExp (ctxt, rgns, e, t, static_eff) ->
+      exists stty',
+        (forall l t', find_ST l stty = Some t' -> find_ST l stty' = Some t')
+         /\ TcHeap (hp', stty')
+         /\ TcVal (stty', v, subst_rho rho t).
+Proof.
+  intros e env rho hp hp' v dynamic_eff HD
+         stty ctxt rgns t static_eff Hhp Hrho Hinc Henv Hexp.
+  destruct (ty_sound_strong e env rho hp hp' v dynamic_eff HD
+              stty ctxt rgns t static_eff Hhp Hrho Hinc Henv Hexp)
+    as [stty' [Hweak [HTcHeap [HTcVal _]]]].
+  exists stty'. intuition.
+Qed.
 
 End TypeSoundness.
-
-
