Proofs/HeapFacts.v
@@ -6,7 +6,6 @@ Require Import Definitions.Values.
 Require Import Definitions.Semantics.
 Require Import Definitions.DynamicActions.
 Require Import Proofs.TypeFacts.
-Require Import Definitions.Axioms.
 
 Import Expressions.
 Import ComputedActions.
@@ -282,6 +281,288 @@ Proof.
   dependent induction H; exists h; econstructor; auto. 
 Qed.
 
+Lemma ReadOnlyPhi_Heap_Step_preserves_readonly:
+  forall phi phi' heap heap',
+    ReadOnlyPhi phi ->
+    (phi, heap) ===> (phi', heap') ->
+    ReadOnlyPhi phi'.
+Proof.
+  intros phi phi' heap heap' HRO HStep.
+  dependent induction HStep; inversion HRO; subst; constructor; eauto.
+Qed.
+
+Lemma ReadOnlyPhi_Heap_Step_preserves_heap:
+  forall phi phi' heap heap',
+    ReadOnlyPhi phi ->
+    (phi, heap) ===> (phi', heap') ->
+    heap ≡@{Heap} heap'.
+Proof.
+  intros phi phi' heap heap' HRO HStep.
+  dependent induction HStep; inversion HRO; subst; try reflexivity; eauto.
+Qed.
+
+Lemma ReadOnlyPhi_Heap_StepsAux_preserves_readonly:
+  forall phi heap phi' heap' n,
+    (phi, heap) =a=>* (phi', heap', n) ->
+    ReadOnlyPhi phi ->
+    ReadOnlyPhi phi'.
+Proof.
+  intros phi heap phi' heap' n HSteps.
+  dependent induction HSteps; intros HRO.
+  - exact HRO.
+  - eapply ReadOnlyPhi_Heap_Step_preserves_readonly; eauto.
+  - eapply IHHSteps2; try reflexivity.
+    eapply IHHSteps1; try reflexivity; assumption.
+Qed.
+
+Lemma ReadOnlyPhi_Heap_StepsAux_preserves_heap:
+  forall phi heap phi' heap' n,
+    (phi, heap) =a=>* (phi', heap', n) ->
+    ReadOnlyPhi phi ->
+    heap ≡@{Heap} heap'.
+Proof.
+  intros phi heap phi' heap' n HSteps.
+  dependent induction HSteps; intros HRO.
+  - reflexivity.
+  - eapply ReadOnlyPhi_Heap_Step_preserves_heap; eauto.
+  - assert (Hheap1 : heap ≡@{Heap} heap'0)
+      by (eapply IHHSteps1; try reflexivity; exact HRO).
+    assert (HRO' : ReadOnlyPhi phi'0)
+      by (eapply ReadOnlyPhi_Heap_StepsAux_preserves_readonly; eauto).
+    assert (Hheap2 : heap'0 ≡@{Heap} heap')
+      by (eapply IHHSteps2; try reflexivity; exact HRO').
+    unfold equiv, heap_equiv in *; subst; reflexivity.
+Qed.
+
+Lemma ReadOnlyPhi_Heap_Steps_preserves_heap:
+  forall phi heap phi' heap',
+    (phi, heap) ==>* (phi', heap') ->
+    ReadOnlyPhi phi ->
+    heap ≡@{Heap} heap'.
+Proof.
+  intros phi heap phi' heap' [n HSteps] HRO.
+  eapply ReadOnlyPhi_Heap_StepsAux_preserves_heap; eauto.
+Qed.
+
+Lemma ReadOnlyEvalPreservesHeap:
+  forall h env rho e h' v phi,
+    (h, env, rho, e) ⇓ (h', v, phi) ->
+    ReadOnlyPhi phi ->
+    h ≡@{Heap} h'.
+Proof.
+  intros h env rho e h' v phi H.
+  dependent induction H; intros HRO; subst; try reflexivity.
+  - inversion HRO; subst.
+    repeat match goal with
+    | HSeq : ReadOnlyPhi (Phi_Seq _ _) |- _ =>
+        inversion HSeq; subst; clear HSeq
+    end.
+    assert (Hhf : h ≡@{Heap} fheap) by (eapply IHBigStep1; try reflexivity; eauto).
+    assert (Hfa : fheap ≡@{Heap} aheap) by (eapply IHBigStep2; try reflexivity; eauto).
+    assert (Hab : aheap ≡@{Heap} h') by (eapply IHBigStep3; try reflexivity; eauto).
+    unfold equiv, heap_equiv in *; subst; reflexivity.
+  - inversion HRO; subst.
+    assert (Hhf : h ≡@{Heap} fheap) by (eapply IHBigStep1; try reflexivity; eauto).
+    assert (Hfb : fheap ≡@{Heap} h') by (eapply IHBigStep2; try reflexivity; eauto).
+    unfold equiv, heap_equiv in *; subst; reflexivity.
+  - inversion HRO; subst.
+    eapply ReadOnlyPhi_Heap_Steps_preserves_heap; eauto.
+  - inversion HRO; subst.
+    assert (Hhc : h ≡@{Heap} cheap) by (eapply IHBigStep1; try reflexivity; eauto).
+    assert (Hct : cheap ≡@{Heap} h') by (eapply IHBigStep2; try reflexivity; eauto).
+    unfold equiv, heap_equiv in *; subst; reflexivity.
+  - inversion HRO; subst.
+    assert (Hhc : h ≡@{Heap} cheap) by (eapply IHBigStep1; try reflexivity; eauto).
+    assert (Hcf : cheap ≡@{Heap} h') by (eapply IHBigStep2; try reflexivity; eauto).
+    unfold equiv, heap_equiv in *; subst; reflexivity.
+  - inversion HRO; subst.
+    match goal with
+    | HAlloc : ReadOnlyPhi (Phi_Elem (DA_Alloc _ _ _)) |- _ =>
+        inversion HAlloc
+    end.
+  - inversion HRO; subst.
+    assert (Hha : h ≡@{Heap} h') by (eapply IHBigStep; try reflexivity; eauto).
+    unfold equiv, heap_equiv in *; subst; reflexivity.
+  - inversion HRO; subst.
+    match goal with
+    | HWrite : ReadOnlyPhi (Phi_Elem (DA_Write _ _ _)) |- _ =>
+        inversion HWrite
+    end.
+  - inversion HRO; subst.
+    assert (Hhl : h ≡@{Heap} lheap) by (eapply IHBigStep1; try reflexivity; eauto).
+    assert (Hlr : lheap ≡@{Heap} h') by (eapply IHBigStep2; try reflexivity; eauto).
+    unfold equiv, heap_equiv in *; subst; reflexivity.
+  - inversion HRO; subst.
+    assert (Hhl : h ≡@{Heap} lheap) by (eapply IHBigStep1; try reflexivity; eauto).
+    assert (Hlr : lheap ≡@{Heap} h') by (eapply IHBigStep2; try reflexivity; eauto).
+    unfold equiv, heap_equiv in *; subst; reflexivity.
+  - inversion HRO; subst.
+    assert (Hhl : h ≡@{Heap} lheap) by (eapply IHBigStep1; try reflexivity; eauto).
+    assert (Hlr : lheap ≡@{Heap} h') by (eapply IHBigStep2; try reflexivity; eauto).
+    unfold equiv, heap_equiv in *; subst; reflexivity.
+  - inversion HRO; subst.
+    assert (Hhl : h ≡@{Heap} lheap) by (eapply IHBigStep1; try reflexivity; eauto).
+    assert (Hlr : lheap ≡@{Heap} h') by (eapply IHBigStep2; try reflexivity; eauto).
+    unfold equiv, heap_equiv in *; subst; reflexivity.
+  - subst. eapply IHBigStep; try reflexivity; constructor.
+  - subst. eapply IHBigStep; try reflexivity; constructor.
+Qed.
+
+Lemma Phi_Heap_Steps_trans :
+  forall phi1 heap1 phi2 heap2 phi3 heap3,
+    (phi1, heap1) ==>* (phi2, heap2) ->
+    (phi2, heap2) ==>* (phi3, heap3) ->
+    (phi1, heap1) ==>* (phi3, heap3).
+Proof.
+  intros phi1 heap1 phi2 heap2 phi3 heap3 [n1 H1] [n2 H2].
+  exists (1 + n1 + n2)%nat.
+  eapply PHT_Trans; eauto.
+Qed.
+
+Lemma Phi_Seq_lift_left :
+  forall phi1 heap phi1' heap' phi2,
+    (phi1, heap) ==>* (phi1', heap') ->
+    (Phi_Seq phi1 phi2, heap) ==>* (Phi_Seq phi1' phi2, heap').
+Proof.
+  intros phi1 heap phi1' heap' phi2 [n HSteps].
+  dependent induction HSteps.
+  - exists 0. constructor.
+  - exists 1. constructor. now constructor.
+  - eapply Phi_Heap_Steps_trans; eauto.
+Qed.
+
+Lemma Phi_Seq_lift_right :
+  forall phi2 heap phi2' heap',
+    (phi2, heap) ==>* (phi2', heap') ->
+    (Phi_Seq Phi_Nil phi2, heap) ==>* (Phi_Seq Phi_Nil phi2', heap').
+Proof.
+  intros phi2 heap phi2' heap' [n HSteps].
+  dependent induction HSteps.
+  - exists 0. constructor.
+  - exists 1. constructor. now constructor.
+  - eapply Phi_Heap_Steps_trans; eauto.
+Qed.
+
+Lemma Phi_Seq_steps :
+  forall phi1 heap heap' phi2 heap'',
+    (phi1, heap) ==>* (Phi_Nil, heap') ->
+    (phi2, heap') ==>* (Phi_Nil, heap'') ->
+    (Phi_Seq phi1 phi2, heap) ==>* (Phi_Nil, heap'').
+Proof.
+  intros phi1 heap heap' phi2 heap'' H1 H2.
+  eapply Phi_Heap_Steps_trans.
+  - eapply Phi_Seq_lift_left; eauto.
+  - eapply Phi_Heap_Steps_trans.
+    + eapply Phi_Seq_lift_right; eauto.
+    + exists 1. constructor. constructor.
+Qed.
+
+Lemma Phi_Par_lift_left :
+  forall phi1 heap phi1' heap' phi2,
+    (phi1, heap) ==>* (phi1', heap') ->
+    (Phi_Par phi1 phi2, heap) ==>* (Phi_Par phi1' phi2, heap').
+Proof.
+  intros phi1 heap phi1' heap' phi2 [n HSteps].
+  dependent induction HSteps.
+  - exists 0. constructor.
+  - exists 1. constructor. now constructor.
+  - eapply Phi_Heap_Steps_trans; eauto.
+Qed.
+
+Lemma Phi_Par_lift_right :
+  forall phi1 phi2 heap phi2' heap',
+    (phi2, heap) ==>* (phi2', heap') ->
+    (Phi_Par phi1 phi2, heap) ==>* (Phi_Par phi1 phi2', heap').
+Proof.
+  intros phi1 phi2 heap phi2' heap' [n HSteps].
+  dependent induction HSteps.
+  - exists 0. constructor.
+  - exists 1. constructor. now constructor.
+  - eapply Phi_Heap_Steps_trans; eauto.
+Qed.
+
+Lemma Phi_Par_steps :
+  forall phi1 heap heap' phi2 heap'',
+    (phi1, heap) ==>* (Phi_Nil, heap') ->
+    (phi2, heap') ==>* (Phi_Nil, heap'') ->
+    (Phi_Par phi1 phi2, heap) ==>* (Phi_Nil, heap'').
+Proof.
+  intros phi1 heap heap' phi2 heap'' H1 H2.
+  eapply Phi_Heap_Steps_trans.
+  - eapply Phi_Par_lift_left; eauto.
+  - eapply Phi_Heap_Steps_trans.
+    + eapply Phi_Par_lift_right; eauto.
+    + exists 1. constructor. constructor.
+Qed.
+
+Lemma BigStep_replays_trace :
+  forall heap env rho e heap' v phi,
+    (heap, env, rho, e) ⇓ (heap', v, phi) ->
+    (phi, heap) ==>* (Phi_Nil, heap').
+Proof.
+  intros heap env rho e heap' v phi HBig.
+  dependent induction HBig; subst; try (exists 0; constructor).
+  - match goal with
+    | HEqual : ?h ≡@{Heap} ?h' |- _ =>
+        unfold equiv, heap_equiv in HEqual; subst h'
+    end.
+    eapply Phi_Seq_steps.
+    + eapply Phi_Seq_steps; eauto.
+    + eauto.
+  - eapply Phi_Seq_steps; eauto.
+  - eapply Phi_Seq_steps.
+    + eapply Phi_Seq_steps; eauto.
+    + eauto.
+  - match goal with
+    | HEqual : ?h ≡@{Heap} ?h1 /\ ?h ≡@{Heap} ?h2 |- _ =>
+        destruct HEqual as [HEq1 HEq2]
+    end.
+    unfold equiv, heap_equiv in HEq1, HEq2; subst.
+    match goal with
+    | HStep : (?h, ?env, ?rho, Eff_App ef1 ea1) ⇓ (?h, Eff theta1, acts_eff1) |- _ =>
+        assert (HEff1Steps : (acts_eff1, h) ==>* (Phi_Nil, h))
+          by (eapply IHHBig1; reflexivity)
+    end.
+    match goal with
+    | HStep : (?h, ?env, ?rho, Eff_App ef2 ea2) ⇓ (?h, Eff theta2, acts_eff2) |- _ =>
+        assert (HEff2Steps : (acts_eff2, h) ==>* (Phi_Nil, h))
+          by (eapply IHHBig2; reflexivity)
+    end.
+    eapply Phi_Seq_steps.
+    + eapply Phi_Par_steps; eauto.
+    + eassumption.
+  - match goal with
+    | HEqual : ?h ≡@{Heap} ?h' |- _ =>
+        unfold equiv, heap_equiv in HEqual; subst h'
+    end.
+    eapply Phi_Seq_steps; eauto.
+  - match goal with
+    | HEqual : ?h ≡@{Heap} ?h' |- _ =>
+        unfold equiv, heap_equiv in HEqual; subst h'
+    end.
+    eapply Phi_Seq_steps; eauto.
+  - eapply Phi_Seq_steps; eauto.
+    exists 1. constructor. constructor.
+  - eapply Phi_Seq_steps; eauto.
+    exists 1. constructor. now constructor.
+  - eapply Phi_Seq_steps.
+    + eapply Phi_Seq_steps; eauto.
+    + exists 1. constructor. constructor. assumption.
+  - eapply Phi_Seq_steps; eauto.
+  - eapply Phi_Seq_steps; eauto.
+  - eapply Phi_Seq_steps; eauto.
+  - eapply Phi_Seq_steps; eauto.
+  - assert (HEq : heap ≡@{Heap} heap')
+      by (eapply EmptyTracePreservesHeap_1; eauto).
+    unfold equiv, heap_equiv in HEq; subst.
+    exists 0. constructor.
+  - assert (HEq : heap ≡@{Heap} heap')
+      by (eapply EmptyTracePreservesHeap_1; eauto).
+    unfold equiv, heap_equiv in HEq; subst.
+    exists 0. constructor.
+  - eapply Phi_Seq_steps; eauto.
+Qed.
+
 Lemma H_same_key_add_twice_1 :
   forall r l r0 l0 v v0 (heap : gmap HeapKey HeapVal), 
     (<[ (r0, l0):=v0 ]> (<[ (r, l):=v ]> heap)) !!  (r0, l0) =
@@ -418,4 +699,3 @@ Proof.
     + assumption.
  - assumption.
 Qed.
-
